closer to memoize

Validator/Hedge/Memoize/Memoize.lean
@@ -2,9 +2,11 @@ import Mathlib.Tactic.SimpRw
 
 import Validator.Std.Decidable
 import Validator.Std.Hedge
+import Validator.Std.Vec
 
 import Validator.Regex.Lang
 import Validator.Regex.Room
+import Validator.Regex.Enter
 import Validator.Regex.Memoize.Memoize
 import Validator.Hedge.Denote
 import Validator.Hedge.Grammar
@@ -38,63 +40,211 @@ namespace Hedge
 --     assumption
 --   pure (Subtype.mk res h)
 
-def Grammar.Memoize.derive [DecidableEq σ] [Hashable σ] [DecidableEq α] [Hashable α] [DecidableEq φ] [Hashable φ] (G: Grammar n φ) (Φ: φ → α → Bool)
-  (r: Regex (φ × Ref n)) (node: Node α): StateMemoize σ { dr: (Regex (φ × Ref n)) // dr = Grammar.Room.derive G Φ r node } :=
-  let nodePred: (param: φ × Ref n) → StateMemoize σ {b: Bool // b = (fun ((labelPred, ref): (φ × Ref n)) =>
+-- def List_foldlMemoize
+--   {α: Type}
+--   [DecidableEq α] [Hashable α]
+--   {β: Type}
+--   [DecidableEq β] [Hashable β]
+--   (f: (b: β) -> (a: α) -> m β)
+--   {σ: Type}
+--   [Monad m]
+--   (init: β) (xs: List α): m {b': m β // b' = List.foldlM f init xs} :=
+--   match xs with
+--   | [] => pure ⟨init, rfl⟩
+--   | (x::xs) => do
+--     let x': { b // b = f init x } := ⟨f init x, rfl⟩
+--     let xs': { b' // b' = List.foldl f (↑x') xs } <- List_foldlMemoize (σ := σ) f x' xs
+--     pure (Subtype.mk xs' (by
+--       obtain ⟨x', hx'⟩ := x'
+--       simp only at xs'
+--       obtain ⟨xs', hxs'⟩ := xs'
+--       simp only
+--       rw [hx'] at hxs'
+--       simp only [List.foldl]
+--       exact hxs'
+--     ))
+
+def Vec.mapM [Monad m] (g: α -> β) (f: (a: α) -> m {res // res = g a})  (xs: Vector α n)
+  : m (Vector β n) :=
+  Vector.mapM (fun a => (·.1) <$> (f a)) xs
+
+def List.mappyM [Monad m] {g: α -> β} (f: (a: α) -> m {res // res = g a}) (xs: List α)
+  : m {ys: (List β) // ys = List.map g xs } :=
+  match xs with
+  | [] => pure ⟨[], rfl⟩
+  | (x::xs') => do
+    let ⟨fx, hfx⟩ <- f x
+    let ⟨fxs, hfxs⟩ <- List.mappyM f xs'
+    pure (Subtype.mk (fx::fxs) (by
+      simp only [List.map]
+      rw [hfx]
+      rw [hfxs]
+    ))
+
+theorem eq (xs ys: Vector α n) (h: Vector.toList xs = Vector.toList ys): xs = ys := by
+  obtain ⟨⟨xs⟩, hxs⟩ := xs
+  obtain ⟨⟨ys⟩, hxs⟩ := ys
+  simp_all
+
+-- @[inline] def mapM [Monad m] (f : α → m β) (xs : Vector α n) : m (Vector β n) := do
+--   go 0 (Nat.zero_le n) #v[]
+-- where
+--   go (k : Nat) (h : k ≤ n) (acc : Vector β k) : m (Vector β n) := do
+--     if h' : k < n then
+--       go (k+1) (by omega) (acc.push (← f xs[k]))
+--     else
+--       return acc.cast (by omega)
+
+theorem take_toList (xs: Vector α l):
+  (Vector.take xs n).toList = List.take n xs.toList := by
+  sorry
+
+theorem push_toList (xs: Vector α n) (x: α):
+  (Vector.push xs x).toList = xs.toList ++ [x] := by
+  sorry
+
+theorem take1_toList (xs: Vector α (n + 1)) (h: k <= n):
+  (List.take (k + 1) xs.toList) = (List.take k (xs.toList)) ++ [xs.get ⟨k, by omega⟩] := by
+  sorry
+
+@[inline] def Vec.mapM' [Monad m] (g: α -> β) (f: (a: α) -> m {res // res = g a}) (xs : Vector α n)
+  : m {ys: (Vector β n) // ys = Vector.map g xs } := do
+  go 0 (Nat.zero_le n) ⟨#v[], by simp⟩
+where
+  go (k : Nat) (h : k ≤ n) (acc : {ys: (Vector β k) // ys = Vector.cast (by omega) (Vector.map g (Vector.take xs k)) })
+    : m {ys: (Vector β n) // ys = Vector.map g xs } := do
+      if h' : k < n then
+        f xs[k] >>=
+          fun xsk =>
+            go (k+1) (by omega) (⟨acc.val.push xsk, by
+              obtain ⟨acc, hacc⟩ := acc
+              simp only
+              rw [hacc]
+              obtain ⟨xsk, hxsk⟩ := xsk
+              simp only
+              rw [hxsk]
+              apply eq
+              rw [Vector.cast_toList]
+              rw [Vector.map_toList]
+              rw [take_toList]
+              rw [push_toList]
+              rw [Vector.cast_toList]
+              rw [Vector.map_toList]
+              rw [take_toList]
+              rw [<- hxsk]
+              -- generalize (xs.toList) = xs'
+              cases n with
+              | zero =>
+                contradiction
+              | succ n' =>
+                rw [take1_toList (h := by omega)]
+                rw [List.map_append]
+                congr
+          ⟩)
+      else
+        return ⟨Vector.cast (by omega) acc.val, by
+          generalize_proofs h1 h2
+          obtain ⟨acc, hacc⟩ := acc
+          simp only
+          rw [hacc]
+          aesop
+        ⟩
+
+-- def Vec.mapM' [Monad m] (g: α -> β) (f: (a: α) -> m {res // res = g a}) (xs: Vector α n)
+--   : m {ys: (Vector β n) // ys = Vector.map g xs } :=
+--   match n with
+--   | 0 =>
+--     (pure ⟨@Vector.nil β, by
+--       apply eq
+--       simp only [Vector.toList]
+--       obtain ⟨⟨xs⟩, hxs⟩ := xs
+--       -- aesop?
+--       simp_all only [Vector.map_mk, List.map_toArray, List.nil_eq, List.map_eq_nil_iff]
+--       simp_all only [List.size_toArray, List.length_eq_zero_iff]
+--     ⟩)
+--   | Nat.succ n' =>
+
+--     sorry
+
+
+--   -- let ys': Vector {(b: β) // b = g } n <- Vector.mapM (fun a => f a) xs
+
+--   -- sorry
+
+def Regex.StateMemoize.deriveM [DecidableEq σ] [Hashable σ]
+  (Φ': σ -> Bool) (Φ: (s: σ) → StateMemoize σ { b // b = Φ' s }) (r: Regex σ):
+  StateMemoize σ {dr: Regex σ // dr = Regex.Room.derive Φ' r } := do
+  let ⟨symbols, hsymbols⟩ <- MemoizeRoom.enterM r
+  let bools <- Vec.mapM' Φ' Φ symbols
+  let ⟨res, hres⟩ <- MemoizeRoom.leaveM ⟨r, bools⟩
+  let h: res = Regex.Room.derive Φ' r := by
+    unfold leave at hres
+    simp only at hres
+    subst_eqs
+    rename_i hleave
+    obtain ⟨bools, hbools⟩ := bools
+    obtain ⟨leave, hleave⟩ := hleave
+    simp only
+    rw [hbools]
+    rfl
+  pure (Subtype.mk res h)
+
+def Grammar.StateMemoize.derive [DecidableEq α] [Hashable α] [DecidableEq φ] [Hashable φ]
+  (G: Grammar n φ) (Φ: φ → α → Bool)
+  (r: Regex (φ × Ref n)) (node: Node α): StateMemoize (φ × Ref n) { dr: (Regex (φ × Ref n)) // dr = Grammar.Room.derive G Φ r node } := do
+  let nodePred: (param: φ × Ref n) → StateMemoize (φ × Ref n) {b: Bool // b = (fun ((labelPred, ref): (φ × Ref n)) =>
       let ⟨label, children⟩ := node
       let childr := if Φ labelPred label then G.lookup ref else Regex.emptyset
       Regex.null (List.foldl (Grammar.Room.derive G Φ) childr children)
     ) param } := (fun ((labelPred, ref): (φ × Ref n)) => do
     let ⟨label, children⟩ := node
     let childr := if Φ labelPred label then G.lookup ref else Regex.emptyset
-    match List_foldlMemoize (Grammar.Memoize.derive G Φ) childr children with
-    | res =>
-      res >>= fun res' => pure (Subtype.mk (Regex.null res') (by
-        simp
+    -- Regex.null <$> List.foldlM (Grammar.Room.derive G Φ) childr children)
 
-
-
-
-
-        subst childr
-
-
-
-
-
-
-        change Regex.null (List.foldl (Grammar.Room.derive G Φ) childr children)
-
-        sorry
-      ))
+    sorry
+    -- match List_foldlMemoize (Grammar.Memoize.derive G Φ) childr children with
+    -- | res =>
+    --   res >>= fun res' => pure (Subtype.mk (Regex.null res') (by
+    --     simp
+    --     subst childr
+    --     -- change Regex.null (List.foldl (Grammar.Room.derive G Φ) childr children)
+    --     sorry
+    --   ))
   )
-  Regex.Room.deriveM nodePred r
-
---  let symbols := enter r
---   let bools <- Vector.mapM Φ symbols
---   pure (leave r bools)
+  let dr <- Regex.StateMemoize.deriveM (fun ((labelPred, ref): (φ × Ref n)) =>
+      let ⟨label, children⟩ := node
+      let childr := if Φ labelPred label then G.lookup ref else Regex.emptyset
+      Regex.null (List.foldl (Grammar.Room.derive G Φ) childr children)
+    ) nodePred r
+  pure (Subtype.mk dr.val (by
+    obtain ⟨dr, hdr⟩ := dr
+    simp only
+    rw [hdr]
+    unfold Grammar.Room.derive
+    rfl
+  ))
 
 def StateMemoize.Grammar.derive.run {φ: Type} [DecidableEq φ] [Hashable φ] [DecidableEq α] [Hashable α]
-  (state: memoizeState φ) (G: Grammar n φ) (Φ: φ → α → Bool) (r: Regex (φ × Ref n)) (node: Node α): Regex (φ × Ref n) :=
-  StateMemoize.run state (Grammar.Memoize.derive G Φ r node)
+  (state: memoizeState (φ × Ref n)) (G: Grammar n φ) (Φ: φ → α → Bool) (r: Regex (φ × Ref n)) (node: Node α): Regex (φ × Ref n) :=
+  StateMemoize.run state (Grammar.StateMemoize.derive G Φ r node)
 
 lemma StateMemoize.Grammar.derive.run_unfold {φ: Type} [DecidableEq φ] [Hashable φ] [DecidableEq α] [Hashable α]
-  (state: memoizeState φ) (G: Grammar n φ) (Φ: φ → α → Bool) (r: Regex (φ × Ref n)) (node: Node α):
-  (StateMemoize.Grammar.derive.run state G Φ r node) = StateMemoize.run state (Grammar.Memoize.derive G Φ r node) :=
+  (state: memoizeState (φ × Ref n)) (G: Grammar n φ) (Φ: φ → α → Bool) (r: Regex (φ × Ref n)) (node: Node α):
+  (StateMemoize.Grammar.derive.run state G Φ r node) = StateMemoize.run state (Grammar.StateMemoize.derive G Φ r node) :=
   rfl
 
 theorem StateMemoize.Grammar.derive.run_is_correct [DecidableEq φ] [Hashable φ] [DecidableEq α] [Hashable α]
-  (state: memoizeState φ)
+  (state: memoizeState (φ × Ref n))
   (Φ: φ → α → Bool) (G: Grammar n φ) (r: Regex (φ × Ref n)) (node: Node α):
   StateMemoize.Grammar.derive.run state G Φ r node = Grammar.Room.derive G Φ r node := by
   rw [StateMemoize.Grammar.derive.run_unfold]
-  generalize StateMemoize.run state (Grammar.Memoize.derive G Φ r node) = x
+  generalize StateMemoize.run state (Grammar.StateMemoize.derive G Φ r node) = x
   obtain ⟨dr, hdr⟩ := x
   simp only
   rw [hdr]
 
 theorem StateMemoize.Grammar.derive_commutes [DecidableEq φ] [Hashable φ] [DecidableEq α] [Hashable α]
-  (state: memoizeState φ)
+  (state: memoizeState (φ × Ref n))
   (Φ: φ → α → Prop) [DecidableRel Φ]
   (G: Grammar n φ) (r: Regex (φ × Ref n)) (node: Node α):
   Grammar.Rule.denote G Φ (StateMemoize.Grammar.derive.run state G (decideRel Φ) r node)
